\chapter{A linguagem da Teoria dos Conjuntos}

\subsection*{Exercício 1}

\begin{enumerate}
	\item[a)] $\neg \exists x \forall y (y \in x) \equiv \forall x \exists y (y \notin x)$
	\item[b)] $\exists ! x \forall y (y \notin x)$
	\item[c)] $\exists ! y (y \in x)$
	\item[d)] $\exists x \forall y ((y \in x) \rightarrow y = \phi)$
	\item[e)] $r \text{ é subconjunto de } x \equiv \forall a ((a \in r) \rightarrow (a \in x)) \equiv A$, então podemos escrever $\forall w ([A]_r^w \leftrightarrow w \in y)$
\end{enumerate}

\subsection*{Exercício 2}

\begin{enumerate}
	\item[a)] $y$
	\item[b)] $y$
	\item[c)] $x$
	\item[d)] Não há variáveis livres.
	\item[e)] $x$ e $y$
\end{enumerate}

\subsection*{Exercício 3}

\begin{enumerate}
	\item 
	\begin{enumerate}
		\item $(\forall x (x = y)) \rightarrow (x \in y)$
		\item $(\forall x (x = y))$
		\item $(x = y)$
		\item $(x \in y)$
	\end{enumerate}
	
	\item 
	\begin{enumerate}
		\item $\forall x ((x = y) \rightarrow (x \in y))$
		\item $(x = y) \rightarrow (x \in y)$
		\item $(x = y)$
		\item $(x \in y)$
	\end{enumerate}
	
	\item 
	\begin{enumerate}
		\item $\forall x (x = x) \rightarrow (\forall y \exists z (((x = y) \land (y = z)) \rightarrow \neg (x \in y)))$
		\item $\forall x (x = x)$
		\item $(x = y)$
		\item $\forall z \exists y (((x = y) \land (y = z)) \rightarrow \neg (x \in y))$
		\item $((x = y) \land (y = z))$
		\item $(x = y)$
		\item $(y = z)$
		\item $\neg (x \in y)$
		\item $(x \in y)$
	\end{enumerate}
	
	\item 
	\begin{enumerate}
		\item $(x = y) \rightarrow \exists y (x = y)$
		\item $(x = y)$
		\item $\exists y (x = y)$
		\item $(x = y)$
	\end{enumerate}
\end{enumerate}